translations/translation_utils.v
@@ -53,14 +53,23 @@ Instance monad_exc : MonadExc tsl_error tsl_result :=
       end
   }.
 
+Definition lookup_tsl_table' E gr :=
+  match lookup_tsl_table E gr with
+  | Some t => ret t
+  | None => raise (TranslationNotFound (string_of_gref gr))
+  end.
 
 
-Class Translation := { tsl_id : ident -> ident ;
-                       tsl_tm : tsl_context -> term -> tsl_result term ;
-                       tsl_ty : tsl_context -> term -> tsl_result term ;
-                       tsl_ind : tsl_context -> kername -> kername -> mutual_inductive_body
-                            -> tsl_result (tsl_table * list mutual_inductive_body)
-                     }.
+
+
+Class Translation :=
+  { tsl_id : ident -> ident ;
+    tsl_tm : tsl_context -> term -> tsl_result term ;
+    tsl_ty : option (tsl_context -> term -> tsl_result term) ;
+
+    (* string = ModPath in which the inductive will be declared *)
+    tsl_ind : tsl_context -> string -> kername -> mutual_inductive_body
+              -> tsl_result (tsl_table * list mutual_inductive_body) }.
 
 
 Definition tsl_ident (id : ident) : ident := (id ++ "ᵗ")%string.
@@ -72,47 +81,57 @@ Definition tsl_name tsl_ident n :=
   end.
 
 
+Definition tmDebug {A} : A -> TemplateMonad unit
+  := tmPrint.
+  (* := fun _ => ret tt. *)
 
-Definition tTranslate {tsl : Translation} (ΣE : tsl_context) (id : ident)
+
+Definition Translate {tsl : Translation} (ΣE : tsl_context) (id : ident)
   : TemplateMonad tsl_context :=
   gr <- tmAbout id ;;
-  id' <- tmEval all (tsl_id id) ;;
-  mp <- tmCurrentModPath tt ;;
-  kn' <- tmEval all (mp ++ "." ++ id') ;;
   match gr with
   | None => fail_nf (id ++ " not found")
   | Some (ConstructRef (mkInd kn n) _)
   | Some (IndRef (mkInd kn n)) =>
-      d <- tmQuoteInductive id ;;
-      d' <- tmEval lazy (tsl_ind ΣE kn kn' d) ;;
-      match d' with
-      | Error e => print_nf e ;; fail_nf ("Translation error during the translation of the inductive " ++ id)
-      | Success (E, decls) =>
-        monad_fold_left (fun _ e => tmMkInductive' e) decls tt ;;
-        let Σ' := add_global_decl (InductiveDecl kn d) (fst ΣE) in
-        let E' := (E ++ (snd ΣE))%list in
-        Σ' <- tmEval lazy Σ' ;;
-        E' <- tmEval lazy E' ;;
-        print_nf  (kn ++ " has been translated as " ++ id') ;;
-        ret (Σ', E')
-      end
-
+    mp <- tmCurrentModPath tt ;;
+    d <- tmQuoteInductive id ;;
+    d' <- tmEval lazy (tsl_ind ΣE mp kn d) ;;
+    match d' with
+    | Error e =>
+      print_nf e ;;
+      fail_nf ("Translation error during the translation of the inductive " ++ id)
+    | Success (E, decls) =>
+      monad_iter tmMkInductive' decls ;;
+      let Σ' := add_global_decl (InductiveDecl kn d) (fst ΣE) in
+      let E' := (E ++ (snd ΣE))%list in
+      Σ' <- tmEval lazy Σ' ;;
+      E' <- tmEval lazy E' ;;
+      print_nf  (kn ++ " has been translated.") ;;
+      ret (Σ', E')
+    end
+    
   | Some (ConstRef kn) =>
     e <- tmQuoteConstant kn true ;;
     match e with
-    | ParameterEntry _ => fail_nf (id ++ "is an axiom, not a definition")
+    | ParameterEntry _ =>
+      fail_nf (id ++ " is an axiom, not a definition. Use Implement Existing.")
     | DefinitionEntry {| definition_entry_type := A;
                          definition_entry_universes := univs;
                          definition_entry_body := t |} =>
+      tmDebug t ;;
       t' <- tmEval lazy (tsl_tm ΣE t) ;;
+      tmDebug t' ;;
       match t' with
-      | Error e => print_nf e ;; fail_nf ("Translation error during the translation of the body of " ++ id)
+      | Error e =>
+        print_nf e ;;
+        fail_nf ("Translation error during the translation of the body of " ++ id)
       | Success t' =>
+        id' <- tmEval all (tsl_id id) ;;
         tmMkDefinition id' t' ;;
         let decl := {| cst_universes := univs;
                        cst_type := A; cst_body := Some t |} in
         let Σ' := add_global_decl (ConstantDecl kn decl) (fst ΣE) in
-        let E' := (ConstRef kn, tConst kn' []) :: (snd ΣE) in
+        let E' := (ConstRef kn, tConst id' []) :: (snd ΣE) in
         Σ' <- tmEval lazy Σ' ;;
         E' <- tmEval lazy E' ;;
         print_nf  (id ++ " has been translated as " ++ id') ;;
@@ -122,18 +141,22 @@ Definition tTranslate {tsl : Translation} (ΣE : tsl_context) (id : ident)
   end.
 
 
-
-Definition tImplement {tsl : Translation} (ΣE : tsl_context)
+Definition Implement {tsl : Translation} (ΣE : tsl_context)
            (id : ident) (A : Type)
   : TemplateMonad (tsl_context) :=
-  tA <- tmQuote A ;;
+  tA  <- tmQuote A ;;
+  match tsl_ty with
+  | None => tmFail "No implementation of tsl_ty provided for this translation."
+  | Some tsl_ty => 
   tA' <- tmEval lazy (tsl_ty ΣE tA) ;;
   print_nf tA' ;;
   match tA' with
-  | Error e => print_nf e ;; fail_nf ("Translation error during the translation of the type of " ++ id)
+  | Error e =>
+    print_nf e ;;
+    tmFail "Translation error during the translation of the type."
   | Success tA' =>
       id' <- tmEval all (tsl_id id) ;;
-      A' <- tmUnquoteTyped Type tA' ;;
+      tmBind (tmUnquoteTyped Type tA') (fun A' =>
       tmLemma id' A' ;;
       tmAxiom id A ;;
       gr <- tmAbout id ;;
@@ -145,8 +168,9 @@ Definition tImplement {tsl : Translation} (ΣE : tsl_context)
         let E' := (ConstRef kn, tConst id' []) :: (snd ΣE) in
         print_nf (id ++ " has been translated as " ++ id') ;;
         ret (Σ', E')
-      | _ => fail_nf (id ++ " was not found or is not a constant, this is a bug")
-      end
+      | _ => fail_nf (id ++ " was not found or is not a constant. This is a bug.")
+      end)
+  end
   end.
 
 Definition body_constant_entry (e : constant_entry) : option term :=
@@ -156,16 +180,14 @@ Definition body_constant_entry (e : constant_entry) : option term :=
   end.
 
 
-Definition tmDebug {A} : A -> TemplateMonad unit
-  (* := tmPrint. *)
-  := fun _ => ret tt.
-
-Definition tImplementExisting {tsl : Translation} (ΣE : tsl_context) (id : ident)
+Definition ImplementExisting {tsl : Translation} (ΣE : tsl_context) (id : ident)
   : TemplateMonad tsl_context :=
   gr <- tmAbout id ;;
   id' <- tmEval all (tsl_id id) ;;
   mp <- tmCurrentModPath tt ;;
-  kn' <- tmEval all (mp ++ "." ++ id') ;;
+  match tsl_ty with
+  | None => tmFail "No implementation of tsl_ty provided for this translation."
+  | Some tsl_ty => 
   match gr with
   | None => fail_nf (id ++ " not found")
   | Some (ConstRef kn) =>
@@ -179,81 +201,78 @@ Definition tImplementExisting {tsl : Translation} (ΣE : tsl_context) (id : iden
       tA' <- tmEval lazy (tsl_ty ΣE A) ;;  (* long *)
       tmDebug "plop" ;;
       match tA' with
-      | Error e => print_nf e ;; fail_nf ("Translation error during the translation of the type of " ++ id)
+      | Error e =>
+        print_nf e ;;
+        fail_nf ("Translation error during the translation of the type of " ++ id)
       | Success tA' =>
-      tmDebug "plop2" ;;
-        id' <- tmEval all (tsl_id id) ;;
-        A' <- tmUnquoteTyped Type tA' ;;
-      tmDebug "plop3" ;;
+        tmDebug "plop2" ;;
+        tmBind (tmUnquoteTyped Type tA') (fun A' =>
+        tmDebug "plop3" ;;
         tmLemma id' A' ;;
         let decl := {| cst_universes := Monomorphic_ctx UContext.empty;
                        cst_type := A; cst_body := body_constant_entry e |} in
         let Σ' := add_global_decl (ConstantDecl kn decl) (fst ΣE) in
         let E' := (ConstRef kn, tConst id' []) :: (snd ΣE) in
         print_nf (id ++ " has been translated as " ++ id') ;;
-        ret (Σ', E')
+        ret (Σ', E'))
       end
     end
   | Some (IndRef (mkInd kn n)) =>
     d <- tmQuoteInductive kn ;;
     match List.nth_error (ind_bodies d) n with
-      | None => tmFail "bug"
+      | None => fail_nf ("The declaration of "
+                          ++ id ++ " has not enough bodies. This is a bug.")
       | Some {| ind_type := A |} => 
       tA' <- tmEval lazy (tsl_ty ΣE A) ;;
       match tA' with
-      | Error e => print_nf e ;; fail_nf ("Translation error during the translation of the type of " ++ id)
+      | Error e =>
+        print_nf e ;;
+        fail_nf ("Translation error during the translation of the type of " ++ id)
       | Success tA' =>
         id' <- tmEval all (tsl_id id) ;;
-        A' <- tmUnquoteTyped Type tA' ;;
+        tmBind (tmUnquoteTyped Type tA') (fun A' =>
         tmLemma id' A' ;;
         let Σ' := add_global_decl (InductiveDecl kn d) (fst ΣE) in
         let E' := (IndRef (mkInd kn n), tConst id' []) :: (snd ΣE) in
         print_nf (id ++ " has been translated as " ++ id') ;;
-        ret (Σ', E')
+        ret (Σ', E'))
       end
-      (* d' <- tmEval lazy (tsl_ind ΣE kn kn' d) ;; *)
-      (* match d' with *)
-      (* | Error e => print_nf e ;; fail_nf ("Translation error during the translation of the inductive " ++ id) *)
-      (* | Success (E, decls) => *)
-      (*   monad_fold_left (fun _ e => tmMkInductive' e) decls tt ;; *)
-      (*   let Σ' := add_global_decl (InductiveDecl kn d) (fst ΣE) in *)
-      (*   let E' := (E ++ (snd ΣE))%list in *)
-      (*   Σ' <- tmEval lazy Σ' ;; *)
-      (*   E' <- tmEval lazy E' ;; *)
-      (*   print_nf  (kn ++ " has been translated as " ++ id') ;; *)
-      (*   ret (Σ', E') *)
     end
 
   | Some (ConstructRef (mkInd kn n) k) =>
     d <- tmQuoteInductive kn ;;
-      tmDebug "plop1" ;;
+    tmDebug "plop1" ;;
     match List.nth_error (ind_bodies d) n with
-      | None => tmFail "bug"
-      | Some {| ind_ctors := ctors |} => 
+    | None => fail_nf ("The declaration of "
+                        ++ id ++ " has not enough bodies. This is a bug.")
+    | Some {| ind_ctors := ctors |} => 
       tmDebug "plop2" ;;
-        match List.nth_error ctors k with
-        | None => tmFail "bug'"
-        | Some (id, ty, _) =>
-      tmDebug "plop3" ;;
-          let A := substl (inds kn [] (* FIXME uctx *) (ind_bodies d)) ty in
-      tmDebug "plop4" ;;
-          tA' <- tmEval lazy (tsl_ty ΣE A) ;;
-      tmDebug "plop5" ;;
-          match tA' with
-          | Error e => print_nf e ;;
-                      fail_nf ("Translation error during the translation of the type of " ++ id)
-          | Success tA' =>
-      tmDebug "plop6" ;;
-            id' <- tmEval all (tsl_id id) ;;
-            A' <- tmUnquoteTyped Type tA' ;;
-      tmDebug "plop7" ;;
-            tmLemma id' A' ;;
-            let E' := (ConstructRef (mkInd kn n) k, tConst id' []) :: (snd ΣE) in
-            print_nf (id ++ " has been translated as " ++ id') ;;
-            ret (fst ΣE, E')
-          end
+      match List.nth_error ctors k with
+      | None => fail_nf ("The body of "
+                          ++ id ++ " has not enough constructors. This is a bug.")
+      | Some (_, ty, _) =>  (* keep id? *)
+        tmDebug "plop3" ;;
+        let A := substl (inds kn [] (* FIXME uctx *) (ind_bodies d)) ty in
+        tmDebug "plop4" ;;
+        tA' <- tmEval lazy (tsl_ty ΣE A) ;;
+        tmDebug "plop5" ;;
+        match tA' with
+        | Error e =>
+          print_nf e ;;
+          fail_nf ("Translation error during the translation of the type of " ++ id)
+        | Success tA' =>
+          tmDebug "plop6" ;;
+          id' <- tmEval all (tsl_id id) ;;
+          tmBind (tmUnquoteTyped Type tA') (fun A' =>
+          tmDebug "plop7" ;;
+          tmLemma id' A' ;;
+          let E' := (ConstructRef (mkInd kn n) k, tConst id' []) :: (snd ΣE) in
+          print_nf (id ++ " has been translated as " ++ id') ;;
+          ret (fst ΣE, E'))
         end
+      end
     end
+  end
   end.
 
 
@@ -288,82 +307,73 @@ Definition split_string (sep : Ascii.ascii) (s : string) : list string :=
 (* Compute (split_string "."%char "eopjqd.qS.E"). *)
 (* Compute (split_string "."%char ""). *)
 
+Definition ident_of_kn (kn : kername) : ident
+  := last (split_string "."%char kn) kn.
+
+Definition tsl_kn (tsl_ident : ident -> ident) (kn : kername) mp
+  := mp ++ "." ++ (tsl_ident (ident_of_kn kn)).
 
 
 
-Definition tTranslateRec {tsl : Translation} (ΣE : tsl_context) {A} (t : A)
-  := 
-      (* gr <- tmAbout id ;; *)
-      (* t <- match gr with *)
-      (*     | Some (ConstRef kn) => *)
-      (*       tmUnquote (tConst kn []) *)
-      (*     | Some (IndRef ind) => *)
-      (*       tmUnquote (tInd ind []) *)
-      (*     | Some (ConstructRef ind n) => *)
-      (*       tmUnquote (tConstruct ind n []) *)
-      (*     | None  => fail_nf (id ++ " was not found") *)
-      (*     end ;; *)
-      (* t' <- tmEval hnf (my_projT2 t) ;; *)
-      (* (* let t' := my_projT2 t in *) *)
-      (* tmPrint t';; *)
-      p <- tmQuoteRec t ;;
-      (* tmPrint p ;; *)
-      tmPrint "~~~~~~~~~~~~~~~~~~" ;;
-      monad_fold_left (
-        fun ΣE decl => print_nf ("Translating " ++ global_decl_ident decl) ;;
-                             (* print_nf ΣE ;; *)
-                    match decl with
-                    | ConstantDecl kn decl =>
-                      match lookup_tsl_table (snd ΣE) (ConstRef kn) with
-                      | Some _ => print_nf (kn ++ " was already translated") ;; ret ΣE
-                      | None => 
-                        match decl with
-                        | {| cst_type := A; cst_body := None; cst_universes := univs |}
-                          => fail_nf (kn ++ " is an axiom")
-                        
-                        | {| cst_type := A; cst_body := Some t; cst_universes := univs |} =>
-                          (* tmPrint "go";; *)
-                          t' <- tmEval lazy (tsl_tm ΣE t) ;;
-                          (* tmPrint "done";; *)
-                          match t' with
-                          | Error e => print_nf e ;; fail_nf ("Translation error during the translation of the body of " ++ kn)
-                          | Success t' =>
-                            let id := last (split_string "."%char kn) kn in
-                            let id' := tsl_ident id in
-                            tmMkDefinition id' t' ;;
-                            let Σ' := add_global_decl (ConstantDecl kn decl) (fst ΣE) in
-                            let E' := (ConstRef kn, tConst id' []) :: (snd ΣE) in
-                            Σ' <- tmEval lazy Σ' ;;
-                            E' <- tmEval lazy E' ;;
-                            print_nf  (id ++ " has been translated as " ++ id') ;;
-                            ret (Σ', E')
-                           end
-                        end
-                      end
+Definition TranslateRec {tsl : Translation} (ΣE : tsl_context) {A} (t : A) := 
+  p <- tmQuoteRec t ;;
+  tmPrint "~~~~~~~~~~~~~~~~~~" ;;
+  monad_fold_left (fun ΣE decl =>
+    print_nf ("Translating " ++ global_decl_ident decl) ;;
+    match decl with
+    | ConstantDecl kn decl =>
+      match lookup_tsl_table (snd ΣE) (ConstRef kn) with
+      | Some _ => print_nf (kn ++ " was already translated") ;; ret ΣE
+      | None => 
+        match decl with
+        | {| cst_body := None |} =>
+          fail_nf (kn ++ " is an axiom. Use Implement Existing.")
+                    
+        | {| cst_type := A; cst_body := Some t; cst_universes := univs |} =>
+          tmDebug "go";;
+          t' <- tmEval lazy (tsl_tm ΣE t) ;;
+          tmDebug "done";;
+          match t' with
+          | Error e =>
+            print_nf e ;;
+            fail_nf ("Translation error during the translation of the body of "
+                       ++ kn)
+          | Success t' =>
+            let id := ident_of_kn kn in
+            let id' := tsl_ident id in
+            tmMkDefinition id' t' ;;
+            let Σ' := add_global_decl (ConstantDecl kn decl) (fst ΣE) in
+            let E' := (ConstRef kn, tConst id' []) :: (snd ΣE) in
+            Σ' <- tmEval lazy Σ' ;;
+            E' <- tmEval lazy E' ;;
+            print_nf  (id ++ " has been translated as " ++ id') ;;
+            ret (Σ', E')
+          end
+        end
+      end
 
-                    | InductiveDecl kn d => 
-                      match lookup_tsl_table (snd ΣE) (IndRef (mkInd kn 0)) with
-                      | Some _ => ret ΣE
-                      | None => 
-                        let id := last (split_string "."%char kn) kn in
-                        let id' := tsl_ident id in
-                        let kn' := tsl_ident kn in
-                        (* tmPrint "go'";; *)
-                        d' <- tmEval lazy (tsl_ind ΣE kn id' d) ;;
-                        (* tmPrint "done'";; *)
-                        match d' with
-                        | Error e => 
-                          print_nf e ;; fail_nf ("Translation error during the translation of the inductive " ++ kn)
-                        | Success (E, decls) =>
-                          monad_fold_left (fun _ e => tmMkInductive' e) decls tt ;;
-                                          let Σ' := add_global_decl (InductiveDecl kn d) (fst ΣE) in
-                                          let E' := (E ++ (snd ΣE))%list in
-                                          Σ' <- tmEval lazy Σ' ;;
-                                          E' <- tmEval lazy E' ;;
-                                          print_nf  (kn ++ " has been translated as " ++ id') ;;
-                                          ret (Σ', E')
-                        end
-                      end
-                    end
-      ) (fst p) ΣE
-.
+    | InductiveDecl kn d => 
+      match lookup_tsl_table (snd ΣE) (IndRef (mkInd kn 0)) with
+      | Some _ => print_nf (kn ++ " was already translated") ;; ret ΣE
+      | None => 
+        tmDebug "go'";;
+        mp <- tmCurrentModPath tt ;;
+        d' <- tmEval lazy (tsl_ind ΣE mp kn d) ;;
+        tmDebug "done'";;
+         match d' with
+         | Error e => 
+           print_nf e ;;
+           fail_nf ("Translation error during the translation of the inductive "
+                      ++ kn)
+         | Success (E, decls) =>
+           monad_iter tmMkInductive' decls ;;
+           let Σ' := add_global_decl (InductiveDecl kn d) (fst ΣE) in
+           let E' := (E ++ (snd ΣE))%list in
+           Σ' <- tmEval lazy Σ' ;;
+           E' <- tmEval lazy E' ;;
+           print_nf  (kn ++ " has been translated.") ;;
+           ret (Σ', E')
+         end
+      end
+    end)
+  (fst p) ΣE.
