translations/tsl_fun.v
@@ -7,10 +7,10 @@ Open Scope list_scope. Open Scope string_scope.
 Local Existing Instance config.default_checker_flags.
 
 Set Primitive Projections.
-Record prod A B := pair { fst : A ; snd : B }.
+Record prod A B := pair { π1 : A ; π2 : B }.
 
-Arguments fst {_ _} _.
-Arguments snd {_ _} _.
+Arguments π1 {_ _} _.
+Arguments π2 {_ _} _.
 Arguments pair {_ _} _ _.
 
 Notation "( x ; y )" := (pair x y) : prod_scope.
@@ -18,7 +18,8 @@ Notation " A × B " := (prod A B) (at level 30) : type_scope.
 
 Quote Definition tprod := prod.
 Quote Definition tpair := @pair.
-Definition prod_ind := Eval compute in match tprod with tInd i _ => i | _ => mkInd "bug: prod not an inductive" 0 end.
+Definition prod_ind := Eval compute in
+  match tprod with tInd i _ => i | _ => mkInd "bug: prod not an inductive" 0 end.
 Definition proj1 (t : term) : term
   := tProj (prod_ind, 2, 0) t.
 Definition proj2 (t : term) : term
@@ -30,12 +31,6 @@ Definition timesBool (A : term) := tApp tprod [A; tbool].
 Definition pairTrue typ tm := tApp tpair [typ; tbool; tm; ttrue].
 
 
-
-Definition lookup_tsl_table' E gr :=
-  match lookup_tsl_table E gr with
-  | Some t => ret t
-  | None => raise (TranslationNotFound (string_of_gref gr))
-  end.
 
 
 Local Instance tit : checker_flags
@@ -49,12 +44,15 @@ Fixpoint tsl_rec (fuel : nat) (Σ : global_context) (E : tsl_table) (Γ : contex
   match t with
   | tRel  n => ret (tRel n)
   | tSort s => ret (tSort s)
+
   | tCast t c A => t' <- tsl_rec fuel Σ E Γ t ;;
                   A' <- tsl_rec fuel Σ E Γ A ;;
                   ret (tCast t' c A')
+
   | tProd n A B => A' <- tsl_rec fuel Σ E Γ A ;;
                   B' <- tsl_rec fuel Σ E (Γ ,, vass n A) B ;;
                   ret (timesBool (tProd n A' B'))
+
   | tLambda n A t => A' <- tsl_rec fuel Σ E Γ A ;;
                     t' <- tsl_rec fuel Σ E (Γ ,, vass n A) t ;;
                     match infer Σ (Γ ,, vass n A) t with
@@ -63,39 +61,46 @@ Fixpoint tsl_rec (fuel : nat) (Σ : global_context) (E : tsl_table) (Γ : contex
                       ret (pairTrue (tProd n A' B') (tLambda n A' t'))
                     | TypeError t => raise (TypingError t)
                     end
+
   | tLetIn n t A u => t' <- tsl_rec fuel Σ E Γ t ;;
                      A' <- tsl_rec fuel Σ E Γ A ;;
                      u' <- tsl_rec fuel Σ E (Γ ,, vdef n t A) u ;;
                      ret (tLetIn n t' A' u')
+
   | tApp t us => t' <- tsl_rec fuel Σ E Γ t ;;
                 monad_fold_left (fun t u => u' <- tsl_rec fuel Σ E Γ u ;;
                                          ret (tApp (proj1 t) [u'])) us t'
+
   | tConst s univs => lookup_tsl_table' E (ConstRef s)
   | tInd i univs => lookup_tsl_table' E (IndRef i)
   | tConstruct i n univs => lookup_tsl_table' E (ConstructRef i n)
   | tProj p t => t' <- tsl_rec fuel Σ E Γ t ;;
                 ret (tProj p t)
-  | tFix bodies n => Γ' <- monad_map (fun '{| dname := na; dtype := ty; dbody := b; rarg := r |} =>
-                                      ty' <- tsl_rec fuel Σ E Γ ty ;;
-                                      ret {| decl_name := na; decl_body := None; decl_type := ty'|})
-                       bodies;;
-                    bodies' <- monad_map (fun '{| dname := na; dtype := ty; dbody := b; rarg := r |} =>
-                                           ty' <- tsl_rec fuel Σ E Γ ty ;;
-                                           b'  <- tsl_rec fuel Σ E (Γ ++ Γ')%list b ;;
-                                           ret {| dname := na; dtype := ty'; dbody := b'; rarg := r |})
-                       bodies ;;
-                    ret (tFix bodies' n)
+
+  | tFix bodies n =>
+    Γ' <- monad_map (fun '{| dname := na; dtype := ty; dbody := b; rarg := r |} =>
+                      ty' <- tsl_rec fuel Σ E Γ ty ;;
+                      ret {| decl_name := na; decl_body := None; decl_type := ty'|})
+                   bodies;;
+    bodies' <- monad_map (fun '{| dname := na; dtype := ty; dbody := b; rarg := r |} =>
+                           ty' <- tsl_rec fuel Σ E Γ ty ;;
+                           b'  <- tsl_rec fuel Σ E (Γ ++ Γ')%list b ;;
+                           ret {| dname := na; dtype := ty';
+                                  dbody := b'; rarg := r |})
+                        bodies ;;
+    ret (tFix bodies' n)
   | _ => raise TranslationNotHandeled (* var evar meta case cofix *)
   end
- end.
+  end.
 
 
 (* Definition recompose_prod (nas : list name) (ts : list term) (u : term) *)
 (*   : term *)
 (*   := let nats := List.combine nas ts in *)
-(*      List.fold_right (fun t u => tProd (Datatypes.fst t) (Datatypes.snd t) u) u nats. *)
+(*      List.fold_right (fun t u => tProd (fst t) (snd t) u) u nats. *)
 
-Definition combine' := fun {A B} l => @List.combine A B (Datatypes.fst l) (Datatypes.snd l).
+Definition combine' {A B} (p : list A * list B)
+  := List.combine  (fst p) (snd p).
 
 
 Fixpoint replace pat u t {struct t} :=
@@ -104,7 +109,8 @@ Fixpoint replace pat u t {struct t} :=
     | tCast t c A => tCast (replace pat u t) c (replace pat u A)
     | tProd n A B => tProd n (replace pat u A) (replace (up pat) (up u) B)
     | tLambda n A t => tLambda n (replace pat u A) (replace (up pat) (up u) t)
-    | tLetIn n t A B => tLetIn n (replace pat u t) (replace pat u A) (replace (up pat) (up u) B)
+    | tLetIn n t A B => tLetIn n (replace pat u t) (replace pat u A)
+                              (replace (up pat) (up u) B)
     | tApp t us => tApp (replace pat u t) (List.map (replace pat u) us)
     | tProj p t => tProj p (replace pat u t)
     | _ => t (* todo *)
@@ -115,10 +121,10 @@ Fixpoint replace pat u t {struct t} :=
 (* a term of type [Π A0 A1 ... . B] *)
 Definition pouet (tm typ : term) : term.
   refine (let L := decompose_prod typ in _).
-  simple refine (let L' := List.fold_left _ (combine' (Datatypes.fst L)) [] in _).
-  exact (fun Γ' A => Γ' ,, vass (Datatypes.fst A) (Datatypes.snd A)).
+  simple refine (let L' := List.fold_left _ (combine' (fst L)) [] in _).
+  exact (fun Γ' A => Γ' ,, vass (fst A) (snd A)).
   refine (let args := fold_left_i (fun l i _ => tRel i :: l) L' [] in _).
-  refine (Datatypes.fst (List.fold_left _ L' (subst_app tm args, Datatypes.snd L))).
+  refine (fst (List.fold_left _ L' (subst_app tm args, snd L))).
   refine (fun '(tm, typ) decl =>
             let A := tProd decl.(decl_name) decl.(decl_type) typ in
             (pairTrue A (tLambda decl.(decl_name) decl.(decl_type) tm),
@@ -127,32 +133,33 @@ Defined.
 
 
 
-Definition tsl_mind_body (ΣE : tsl_context) (kn kn' : kername)
+Definition tsl_mind_body (ΣE : tsl_context) (mp : string) (kn : kername)
            (mind : mutual_inductive_body)
   : tsl_result (tsl_table * list mutual_inductive_body).
-  refine (let tsl := fun Γ t => match tsl_rec fuel (Datatypes.fst ΣE) (Datatypes.snd ΣE) Γ t with
+  refine (let tsl := fun Γ t => match tsl_rec fuel (fst ΣE) (snd ΣE) Γ t with
                              | Success x => x
                              | Error _ => todo
-                             end in _).
+                             end in
+          let kn' := tsl_kn tsl_ident kn mp in _).
   refine (let LI := List.split (map_i _ mind.(ind_bodies)) in
-          ret (List.concat (Datatypes.fst LI),
+          ret (List.concat (fst LI),
                [{| ind_npars := mind.(ind_npars);
-                   ind_bodies := Datatypes.snd LI;
+                   ind_bodies := snd LI;
                    ind_universes := mind.(ind_universes)|}])). (* FIXME always ok? *)
   intros i ind.
   simple refine (let ind_type' := _ in
                  let ctors' := List.split (map_i _ ind.(ind_ctors)) in
-                 (_ :: Datatypes.fst ctors',
+                 (_ :: fst ctors',
                   {| ind_name := tsl_ident ind.(ind_name);
                      ind_type := ind_type';
                      ind_kelim := ind.(ind_kelim);
-                     ind_ctors := Datatypes.snd ctors';
+                     ind_ctors := snd ctors';
                      ind_projs := [] |})).
   + (* arity *)
     refine (let L := decompose_prod ind.(ind_type) in _).
-    simple refine (let L' := List.fold_left _ (combine' (Datatypes.fst L)) [] in _).
-    exact (fun Γ' A => Γ' ,, vass (Datatypes.fst A) (tsl Γ' (Datatypes.snd A))).
-    refine (List.fold_left _ L' (Datatypes.snd L)).
+    simple refine (let L' := List.fold_left _ (combine' (fst L)) [] in _).
+    exact (fun Γ' A => Γ' ,, vass (fst A) (tsl Γ' (snd A))).
+    refine (List.fold_left _ L' (snd L)).
     exact (fun t decl => tProd decl.(decl_name) decl.(decl_type) t).
   + (* constructors *)
     intros k ((name, typ), nargs).
@@ -163,11 +170,12 @@ Definition tsl_mind_body (ΣE : tsl_context) (kn kn' : kername)
     * refine (fold_left_i (fun t i _ => replace (proj1 (tRel i)) (tRel i) t)
                           mind.(ind_bodies) _).
       refine (let L := decompose_prod typ in _).
-      simple refine (let L' := List.fold_left _ (combine' (Datatypes.fst L)) [] in _).
-      exact (fun Γ' A => Γ' ,, vass (Datatypes.fst A) (tsl Γ' (Datatypes.snd A))).
+      simple refine (let L' := List.fold_left _ (combine' (fst L))
+                                              [] in _).
+      exact (fun Γ' A => Γ' ,, vass (fst A) (tsl Γ' (snd A))).
       refine (List.fold_left _ L' _).
       exact (fun t decl => tProd decl.(decl_name) decl.(decl_type) t).
-      exact (match Datatypes.snd L with
+      exact (match snd L with
              | tApp t us => tApp t (List.map (tsl L') us)
              | _ as t => t
              end).
@@ -181,22 +189,24 @@ Open Scope prod_scope.
 
 Instance tsl_fun : Translation
   := {| tsl_id := tsl_ident ;
-        tsl_tm := fun ΣE => tsl_rec fuel (Datatypes.fst ΣE) (Datatypes.snd ΣE) [] ;
-        tsl_ty := fun ΣE => tsl_rec fuel (Datatypes.fst ΣE) (Datatypes.snd ΣE) [] ;
+        tsl_tm := fun ΣE => tsl_rec fuel (fst ΣE) (snd ΣE) [] ;
+        tsl_ty := Some (fun ΣE => tsl_rec fuel (fst ΣE) (snd ΣE) []) ;
         tsl_ind := tsl_mind_body |}.
 
 
-Tactic Notation "tSpecialize" ident(H) uconstr(t) := apply fst in H; specialize (H t).
+Tactic Notation "tSpecialize" ident(H) uconstr(t)
+  := apply π1 in H; specialize (H t).
+Tactic Notation "tIntro" ident(H)
+  := refine (fun H => _; true).
 
-Tactic Notation "tIntro" ident(H) := refine (fun H => _; true).
+Definition NotFunext :=
+  ((forall (A B : Set) (f g : A -> B), (forall x:A, f x = g x) -> f = g) -> False).
 
-Run TemplateProgram (TC <- tTranslate emptyTC "eq" ;;
-                     TC <- tTranslate TC "False" ;;
+Run TemplateProgram (TC <- TranslateRec emptyTC NotFunext ;;
                      tmDefinition "TC" TC ;;
-                     tImplement TC "notFunext"
-                     ((forall (A B : Set) (f g : A -> B), (forall x:A, f x = g x) -> f = g) -> False)).
-
-Next Obligation.
+                     Implement TC "notFunext" NotFunext).
+Next Obligation. 
+  unfold NotFunextᵗ; cbn in *.
   tIntro H. 
   tSpecialize H unit. tSpecialize H unit. 
   tSpecialize H (fun x => x; true). tSpecialize H (fun x => x; false). 
@@ -204,7 +214,7 @@ Next Obligation.
   inversion H. 
 Defined.
 
-Run TemplateProgram (tImplement TC "notη" ((forall (A B : Set) (f : A -> B), f = fun x => f x) -> False)).
+Run TemplateProgram (Implement TC "notη" ((forall (A B : Set) (f : A -> B), f = fun x => f x) -> False)).
 
 Next Obligation.
   tIntro H. 
@@ -214,11 +224,15 @@ Next Obligation.
 Defined.
 
 Require Import Vector Even.
-(* Run TemplateProgram (TC <- tTranslate emptyTC "nat" ;; *)
-(*                      TC <- tTranslate TC "t" ;; *)
-(*                      TC <- tTranslate TC "even" ;; ret tt). *)
+Definition SS := S.
+Run TemplateProgram (TC <- Translate emptyTC "nat" ;;
+                     TC <- Translate TC "even" ;;
+                     tmDefinition "TC2" TC).
 
-
+Inductive foo :=
+| bar : (nat -> foo) -> foo.
+Definition bar' := bar.
+Run TemplateProgram (TranslateRec TC2 bar').
 
 Require Import MiniHoTT.
 Module Axioms.
@@ -228,7 +242,7 @@ Module Axioms.
 
   Run TemplateProgram (tmQuoteRec UIP >>= tmPrint).
 
-  Run TemplateProgram (TC <- tTranslateRec emptyTC UIP ;;
+  Run TemplateProgram (TC <- TranslateRec emptyTC UIP ;;
                        tmDefinition "eqTC" TC).
 
   Definition eqᵗ_eq {A} x y
@@ -267,9 +281,9 @@ Module Axioms.
  
 
   Open Scope prod_scope.
-  Run TemplateProgram (TC <- tTranslateRec eqTC (wFunext -> False) ;;
+  Run TemplateProgram (TC <- TranslateRec eqTC (wFunext -> False) ;;
                        tmDefinition "eqTC'" TC ;;
-                       tImplement TC "notwFunext" (wFunext -> False)).
+                       Implement TC "notwFunext" (wFunext -> False)).
   Next Obligation.
     tIntro H.
     tSpecialize H unit. tSpecialize H (fun _ => unit; true). 
@@ -281,16 +295,16 @@ Module Axioms.
   Definition wUnivalence
     := forall A B, Equiv A B -> A = B.
  
-  Run TemplateProgram (TC <- tTranslate eqTC' "idpath" ;;
-                            TC <- tImplementExisting TC "paths_ind" ;;
+  Run TemplateProgram (TC <- Translate eqTC' "idpath" ;;
+                            TC <- ImplementExisting TC "paths_ind" ;;
                             tmDefinition "eqTC''" TC).
   Next Obligation.
     tIntro A. tIntro a. tIntro P. tIntro t.
     tIntro y. tIntro p. destruct p. exact t.
   Defined.
 
-  Run TemplateProgram (TC <- tTranslateRec eqTC'' (wUnivalence -> False) ;;
-                       tImplement TC "notwUnivalence" (wUnivalence -> False)).
+  Run TemplateProgram (TC <- TranslateRec eqTC'' (wUnivalence -> False) ;;
+                       Implement TC "notwUnivalence" (wUnivalence -> False)).
   Next Obligation.
   Admitted.
 
